unusedglob/VerComp.v
@@ -1,0 +1,287 @@
+Require Import Relations.
+Require Import Wellfounded.
+Require Import Coqlib.
+Require Import Events.
+Require Import Globalenvs.
+Require Import LanguageInterface.
+Require Import Integers.
+Require Import Memory.
+Require Import Smallstep.
+Require Import Inject InjectFootprint.
+Require Import Callconv ForwardSim.
+
+(** * Test1: compose injp' ⋅ injp' = injp' *)
+
+(*
+L1 <=injp'->injp' L2 ->
+L2 <=injp'->injp' L3 ->
+L1 <= injp'-> injp' L3
+*)
+
+Section COMPOSE_FORWARD_SIMULATIONS.
+
+Context (L1: semantics li_c li_c) (L2: semantics li_c li_c) (L3: semantics li_c li_c).
+
+Definition symtbl_dom (se: Genv.symtbl) : meminj :=
+  fun b => if Mem.sup_dec b (Genv.genv_sup se) then Some (b,0)
+        else None.
+
+Definition source_inj (se: Genv.symtbl) (f : meminj) :=
+  fun b => if Mem.sup_dec b (Genv.genv_sup se) then
+        Some (b,0) else meminj_dom f b.
+
+Lemma source_inj_meminj_dom_incr : forall se f,
+    inject_incr (meminj_dom f) (source_inj se f).
+Proof.
+  intros. intro. intros.
+  unfold source_inj.
+  unfold meminj_dom in *.
+  destruct (f b); try discriminate. inv H.
+  destruct Mem.sup_dec; eauto.
+Qed.
+
+Global Instance source_inj_incr se:
+  Monotonic (@source_inj se) (inject_incr ++> inject_incr).
+Proof.
+  intros f g Hfg b b' delta Hb.
+  unfold source_inj in *.
+  destruct (Mem.sup_dec). eauto.
+  eapply meminj_dom_incr; eauto.
+Qed.
+
+Lemma source_inj_compose se f:
+  compose_meminj (source_inj se f) f = f.
+Proof.
+  apply Axioms.functional_extensionality; intros b.
+  unfold compose_meminj, source_inj, meminj_dom.
+  destruct (Mem.sup_dec).
+  destruct (f b) as [[b' ofs] | ] eqn:Hfb; eauto.
+  destruct (f b) as [[b' ofs] | ] eqn:Hfb; eauto.
+  rewrite Hfb.
+  replace (0 + ofs) with ofs by extlia.
+  reflexivity.
+Qed.
+
+Lemma block_inject_dom se f b1 b2:
+  block_inject f b1 b2 ->
+  block_inject (source_inj se f) b1 b1.
+Proof.
+  unfold source_inj,meminj_dom.
+  intros (delta & Hb).
+  exists 0.
+  rewrite Hb; eauto.
+  destruct Mem.sup_dec; eauto.
+Qed.
+
+Lemma val_inject_dom se f v1 v2:
+  Val.inject f v1 v2 ->
+  Val.inject (source_inj se f) v1 v1.
+Proof.
+  destruct 1; econstructor.
+  - unfold source_inj, meminj_dom.
+    rewrite H. destruct Mem.sup_dec; eauto.
+  - rewrite Ptrofs.add_zero.
+    reflexivity.
+Qed.
+
+Lemma memval_inject_dom se f v1 v2:
+  memval_inject f v1 v2 ->
+  memval_inject (source_inj se f) v1 v1.
+Proof.
+  destruct 1; econstructor.
+  eapply val_inject_dom; eauto.
+Qed.
+
+Lemma val_inject_list_dom se f vs1 vs2:
+  Val.inject_list f vs1 vs2 ->
+  Val.inject_list (source_inj se f) vs1 vs1.
+Proof.
+  induction 1; constructor; eauto using val_inject_dom.
+Qed.
+
+Lemma mem_mem_inj_dom se f m1 m2:
+  Mem.mem_inj f m1 m2 ->
+  Mem.mem_inj (source_inj se f) m1 m1.
+Proof.
+  intros H.
+  split.
+  - unfold source_inj, meminj_dom. intros b1 b2 delta ofs k p Hb1 Hp.
+    destruct Mem.sup_dec; destruct (f b1); inv Hb1;
+    replace (ofs + 0) with ofs by extlia; auto.
+  - unfold source_inj, meminj_dom. intros b1 b2 delta chunk ofs p Hb1 Hrp.
+    destruct (Mem.sup_dec); destruct (f b1) as [[b1' delta'] | ]; inv Hb1;
+    eauto using Z.divide_0_r.
+  - unfold source_inj, meminj_dom at 1. intros b1 ofs b2 delta Hb1 Hp.
+    destruct (Mem.sup_dec) eqn:Hs; destruct (f b1) as [[b1' delta'] | ] eqn:Hb1'; inv Hb1.
+    replace (ofs + 0) with ofs by extlia.
+    eapply memval_inject_dom.
+    eapply Mem.mi_memval; eauto.
+    replace (ofs + 0) with ofs by extlia.
+    {
+      set (mv:= (Maps.ZMap.get ofs (NMap.get (Maps.ZMap.t memval) b2 (Mem.mem_contents m1)))).
+      destruct mv; constructor.
+      destruct v; econstructor.
+      rewrite pred_dec_true. 2: eauto.
+    }
+    rewrite pred_dec_true. 2: eauto.
+    Search memval_inject.
+    eapply memval_inject_dom. admit.
+    replace (ofs + 0) with ofs by extlia.
+    eapply memval_inject_dom.
+    eapply Mem.mi_memval; eauto.
+Qed.
+
+Lemma mem_inject_dom f m1 m2:
+  Mem.inject f m1 m2 ->
+  Mem.inject (meminj_dom f) m1 m1.
+Proof.
+  intros H.
+  split.
+  - eapply mem_mem_inj_dom.
+    eapply Mem.mi_inj; eauto.
+  - unfold meminj_dom. intros.
+    erewrite Mem.mi_freeblocks; eauto.
+  - unfold meminj_dom; intros.
+    destruct (f b) as [[b'' delta'] | ] eqn:Hb; inv H0.
+    eapply Mem.valid_block_inject_1; eauto.
+  - red. unfold meminj_dom. intros.
+    destruct (f b1); inv H1.
+    destruct (f b2); inv H2.
+    eauto.
+  - unfold meminj_dom. intros.
+    destruct (f b); inv H0.
+    split; try extlia.
+    rewrite Z.add_0_r.
+    apply Ptrofs.unsigned_range_2.
+  - unfold meminj_dom. intros.
+    destruct (f b1); inv H0.
+    rewrite Z.add_0_r in H1; eauto.
+Qed.
+
+Lemma match_stbls_dom f se1 se2:
+  Genv.match_stbls f se1 se2 ->
+  Genv.match_stbls (meminj_dom f) se1 se1.
+Proof.
+  intros Hse. unfold meminj_dom. split; eauto; intros.
+  - edestruct Genv.mge_dom as (b2 & Hb2); eauto. rewrite Hb2. eauto.
+  - edestruct Genv.mge_dom as (b3 & Hb3); eauto. exists b2. rewrite Hb3. eauto.
+  - destruct (f b1) as [[xb2 xdelta] | ] eqn:Hb; inv H. reflexivity.
+  - destruct (f b1) as [[xb2 xdelta] | ] eqn:Hb; inv H. reflexivity.
+  - destruct (f b1) as [[xb2 xdelta] | ] eqn:Hb; inv H. reflexivity.
+Qed.
+
+Lemma loc_unmapped_dom f b ofs:
+  loc_unmapped (meminj_dom f) b ofs <->
+  loc_unmapped f b ofs.
+Proof.
+  unfold meminj_dom, loc_unmapped.
+  destruct (f b) as [[b' delta] | ].
+  - split; discriminate.
+  - reflexivity.
+Qed.
+
+Lemma mem_inject_source : forall f m1 m2 se,
+    Mem.inject f m1 m2 ->
+    Mem.inject (source_inj se f) m1 m1.
+Proof.
+  intros.
+  exploit mem_inject_dom; eauto.
+  intro.
+  Search Mem.inject.
+Definition soucr_world (w: injp_world) (se:Genv.symtbl) :=
+  match w with
+  |injpw f m1 m2 Hm =>
+     injpw (source_inj se f) m1 m1 (mem_inject_dom f m1 m2 Hm)
+  end.
+
+Lemma match_stbls_dom' f se1 se2:
+  Genv.match_stbls' f se1 se2 ->
+  Genv.match_stbls (meminj_dom f) se1 se1.
+Proof.
+  intros Hse. unfold meminj_dom. split; eauto; intros.
+  - inv Hse.
+  - inv Hse. admit
+  - destruct (f b1) as [[xb2 xdelta] | ] eqn:Hb; inv H. reflexivity.
+  - destruct (f b1) as [[xb2 xdelta] | ] eqn:Hb; inv H. reflexivity.
+  - destruct (f b1) as [[xb2 xdelta] | ] eqn:Hb; inv H. reflexivity.
+Qed.
+
+Lemma compose_fsim_components':
+  fsim_components' (cc_c' injp') (cc_c' injp') L1 L2 ->
+  fsim_components' (cc_c' injp') (cc_c' injp') L2 L3 ->
+  fsim_components' (cc_c' injp') (cc_c' injp') L1 L3.
+Proof.
+  intros [index order match_states Hsk props order_wf].
+  intros [index' order' match_states' Hsk' props' order_wf'].
+  set (ff_index := (index' * index)%type).
+  set (ff_order := lex_ord (clos_trans _ order') order).
+  set (ff_match_states :=
+         fun se1 se3 (w: injp_world) (i: ff_index) (s1: state L1) (s3: state L3) =>
+           exists s2,
+             match_states se1 se1 (id_world w) (snd i) s1 s2 /\
+             match_states' se1 se3 w (fst i) s2 s3).
+  apply Forward_simulation' with ff_order ff_match_states.
+  3: { unfold ff_order. auto using wf_lex_ord, wf_clos_trans. }
+  1: { etransitivity; eauto. }
+  intros se1 se2 w Hse2 Hcompat. cbn in *.
+  assert (Hse1: injp_match_stbls' (id_world w) se1 se1).
+  { clear - Hse2.
+    inv Hse2. constructor; eauto.
+    inv H. constructor; intros; eauto.
+    - unfold meminj_dom in H2. destruct (f b1); try discriminate
+    
+  }
+  assert (Hse1: Genv.valid_for (skel L1) se1).
+  {}
+  Search Genv.skel_le.
+  { rewrite <- Hsk. eapply match_senv_valid_for; eauto. }
+  constructor.
+- (* valid query *)
+  intros q1 q3 (q2 & Hq12 & Hq23).
+  erewrite fsim_match_valid_query by eauto.
+  eapply fsim_match_valid_query; eauto.
+- (* initial states *)
+  intros q1 q3 s1 (q2 & Hq12 & Hq23) Hs1.
+  edestruct (@fsim_match_initial_states liA1) as (i & s2 & A & B); eauto.
+  edestruct (@fsim_match_initial_states liA2) as (i' & s3 & C & D); eauto.
+  exists (i', i); exists s3; split; auto. exists s2; auto.
+- (* final states *)
+  intros. cbn. destruct H as (s3 & A & B).
+  edestruct (@fsim_match_final_states liA1) as (r2 & Hr2 & Hr12); eauto.
+  edestruct (@fsim_match_final_states liA2) as (r3 & Hr3 & Hr23); eauto.
+- (* external states *)
+  intros. destruct H as [s3 [A B]].
+  edestruct (@fsim_match_external liA1) as (w12 & q2 & Hq2 & Hq12 & Hw12 & Hk12); eauto.
+  edestruct (@fsim_match_external liA2) as (w23 & q3 & Hq3 & Hq23 & Hw23 & Hk23); eauto.
+  exists (se2, w12, w23), q3. cbn; repeat apply conj; eauto.
+  intros r1 r3 s1' (r2 & Hr12 & Hr23) Hs1'.
+  edestruct Hk12 as (i12' & s2' & Hs2' & Hs12'); eauto.
+  edestruct Hk23 as (i23' & s3' & Hs3' & Hs23'); eauto.
+  exists (i23', i12'), s3'. split; auto. exists s2'; auto.
+- (* simulation *)
+  intros. destruct H0 as [s3 [A B]]. destruct i as [i2 i1]; simpl in *.
+  edestruct (@fsim_simulation' liA1) as [(i1' & s3' & C & D) | (i1' & C & D & E)]; eauto.
++ (* L2 makes one or several steps. *)
+  edestruct (@simulation_plus liA2) as [(i2' & s2' & P & Q) | (i2' & P & Q & R)]; eauto.
+* (* L3 makes one or several steps *)
+  exists (i2', i1'); exists s2'; split. auto. exists s3'; auto.
+* (* L3 makes no step *)
+  exists (i2', i1'); exists s2; split.
+  right; split. subst t; apply star_refl. red. left. auto.
+  exists s3'; auto.
++ (* L2 makes no step *)
+  exists (i2, i1'); exists s2; split.
+  right; split. subst t; apply star_refl. red. right. auto.
+  exists s3; auto.
+Qed.
+
+Lemma compose_forward_simulations:
+  forward_simulation ccA12 ccB12 L1 L2 ->
+  forward_simulation ccA23 ccB23 L2 L3 ->
+  forward_simulation (ccA12 @ ccA23) (ccB12 @ ccB23) L1 L3.
+Proof.
+  intros [X] [Y]. constructor.
+  apply compose_fsim_components; auto.
+Qed.
+
+End COMPOSE_FORWARD_SIMULATIONS.
